Improve term reconstruction tactic

lava/out/Benchmark/Overview.v
@@ -85,7 +85,7 @@ Definition llen_spec (l : IList): Type :=
 Definition llen (l : IList): llen_spec l.
 Proof.
   destruct l as [l l_p].
-  induction l as [ds_d27L l' IH_l'|].
+  induction l as [ds_d27I l' IH_l'|].
   - refine (subsumptionCast
             Z
             (λ (v : Z), gebZ_rel v 0 true)
@@ -104,9 +104,9 @@ Proof.
 Defined.
 
 Inductive llen_rel: IList_u → Z → Prop :=
-  | llen_Cons: ∀ ds_d27L l' (llen_res : Z),
+  | llen_Cons: ∀ ds_d27I l' llen_res,
                llen_rel l' llen_res
-               → ∀ (addZ_res : Z), addZ_rel llen_res 1 addZ_res → llen_rel (Cons_u ds_d27L l') addZ_res
+               → ∀ addZ_res, addZ_rel llen_res 1 addZ_res → llen_rel (Cons_u ds_d27I l') addZ_res
   | llen_Nil: llen_rel Nil_u 0.
 
 #[global] Hint Constructors llen_rel: core_hint_db.
@@ -117,16 +117,15 @@ Inductive llen_rel: IList_u → Z → Prop :=
 
 Theorem llen_rel_funct [l : IList_u]: ∀ (v v' : Z), llen_rel l v → (llen_rel l v' → v = v').
 Proof.
-  induction l as [ds_d27L l' IH_l'|]; rel_functionhood_body.
+  induction l as [ds_d27I l' IH_l'|]; rel_functionhood_body.
 Qed.
 
 #[global] Hint Resolve llen_rel_funct: f_rel_funct_db.
 
-Theorem llen_Cons_lem ds_d27L l' llen_Cons_lem_res:
-  llen_rel (Cons_u ds_d27L l') llen_Cons_lem_res
-  ↔ ∃ (llen_res : Z),
-    llen_rel l' llen_res
-    ∧ ∃ (addZ_res : Z), addZ_rel llen_res 1 addZ_res ∧ llen_Cons_lem_res == addZ_res.
+Theorem llen_Cons_lem ds_d27I l' llen_Cons_lem_res:
+  llen_rel (Cons_u ds_d27I l') llen_Cons_lem_res
+  ↔ ∃ llen_res,
+    llen_rel l' llen_res ∧ ∃ addZ_res, addZ_rel llen_res 1 addZ_res ∧ llen_Cons_lem_res == addZ_res.
 Proof.
   rel_back' _nil.
 Qed.
@@ -144,12 +143,14 @@ Theorem llen_rel_ex (l : IList_u) (l_p : IList_wf l ∧ True): llen_rel l ⌊ ll
 Proof.
   Opaque llen.
   existence_lemma_pre llen;
-  induction l as [ds_d27L l' IH_l'|];
+  induction l as [ds_d27I l' IH_l'|];
   [fix_notations; pose proof (IH_l' ltac:(try clear IH_l'; solver)) as IH_91252151; try clear IH_l' |
    fix_notations];
   simpl in *.
   Transparent llen.
-  all: (existence_lemma_quicksolve llen; f__f_rel_ex_body; f_rel_finish).
+  all: existence_lemma_quicksolve llen.
+  f__f_rel_ex_body.
+  f_rel_finish.
 Qed.
 
 #[global] Hint Resolve llen_rel_ex: rel_ax_db.
@@ -212,13 +213,13 @@ Defined.
 
 Definition append_spec (xs ys : IList): Type :=
   {v: IList_u | IList_wf v
-                ∧ ∃ (llen_res : Z),
+                ∧ ∃ llen_res,
                   llen_rel v llen_res
-                  ∧ ∃ (llen_res_2 : Z),
+                  ∧ ∃ llen_res_2,
                     llen_rel ⌊ xs ⌋ llen_res_2
-                    ∧ ∃ (llen_res_3 : Z),
+                    ∧ ∃ llen_res_3,
                       llen_rel ⌊ ys ⌋ llen_res_3
-                      ∧ ∃ (addZ_res : Z), addZ_rel llen_res_2 llen_res_3 addZ_res ∧ llen_res == addZ_res}.
+                      ∧ ∃ addZ_res, addZ_rel llen_res_2 llen_res_3 addZ_res ∧ llen_res == addZ_res}.
 
 #[global] Hint Unfold append_spec: lia_unfold.
 
@@ -227,17 +228,17 @@ Proof.
   destruct xs as [xs xs_p].
   destruct ys as [ys ys_p].
   try revert ys_p; generalize dependent ys; induction xs as [x xs IH_xs|]; intros.
-  - refine (subsumptionCast
+  - unfold append_spec. simpl.
+    refine (subsumptionCast
             IList_u
             (λ (v : IList_u),
              IList_wf v
-             ∧ ∃ (llen_res : Z),
+             ∧ ∃ llen_res,
                llen_rel v llen_res
-               ∧ ∃ (llen_res_2 : Z),
-                 llen_rel xs llen_res_2
-                 ∧ ∃ (llen_res_3 : Z),
-                   llen_rel ys llen_res_3
-                   ∧ ∃ (addZ_res : Z), addZ_rel llen_res_2 llen_res_3 addZ_res ∧ llen_res == addZ_res)
+               ∧ ∃ llen_res_2,
+                 llen_rel (Cons_u x xs) llen_res_2
+                 ∧ ∃ llen_res_3,
+                   llen_rel ys llen_res_3 ∧ ∃ addZ_res, addZ_rel llen_res_2 llen_res_3 addZ_res ∧ llen_res == addZ_res)
             (Cons
              (exist (λ (n : Z), ltbZ_rel 5 n true) x ltac:(solver))
              (subsumptionCast
@@ -250,19 +251,18 @@ Proof.
             IList_u
             (λ (v : IList_u),
              IList_wf v
-             ∧ ∃ (llen_res : Z),
+             ∧ ∃ llen_res,
                llen_rel v llen_res
-               ∧ ∃ (llen_res_2 : Z),
-                 llen_rel xs llen_res_2
-                 ∧ ∃ (llen_res_3 : Z),
-                   llen_rel ys llen_res_3
-                   ∧ ∃ (addZ_res : Z), addZ_rel llen_res_2 llen_res_3 addZ_res ∧ llen_res == addZ_res)
+               ∧ ∃ llen_res_2,
+                 llen_rel Nil_u llen_res_2
+                 ∧ ∃ llen_res_3,
+                   llen_rel ys llen_res_3 ∧ ∃ addZ_res, addZ_rel llen_res_2 llen_res_3 addZ_res ∧ llen_res == addZ_res)
             (exist (λ (ys : IList_u), IList_wf ys ∧ True) ys ltac:(solver))
             ltac:(solver)).
 Defined.
 
 Inductive append_rel: IList_u → IList_u → IList_u → Prop :=
-  | append_Cons_x: ∀ x xs ys (append_res : IList_u),
+  | append_Cons_x: ∀ x xs ys append_res,
                    append_rel xs ys append_res → append_rel (Cons_u x xs) ys (Cons_u x append_res)
   | append_Nil_x: ∀ ys, append_rel Nil_u ys ys.
 
@@ -283,8 +283,7 @@ Qed.
 
 Theorem append_Cons_x_lem x xs ys append_Cons_x_lem_res:
   append_rel (Cons_u x xs) ys append_Cons_x_lem_res
-  ↔ ∃ (append_res : IList_u),
-    append_rel xs ys append_res ∧ append_Cons_x_lem_res == Cons_u x append_res.
+  ↔ ∃ append_res, append_rel xs ys append_res ∧ append_Cons_x_lem_res == Cons_u x append_res.
 Proof.
   rel_back' _nil.
 Qed.
@@ -371,13 +370,13 @@ Qed.
      (v_x_62265989 : IList_u),
    ltac:(flattenP (λ (xs ys : IList) (v : IList_u),
  IList_wf v
- ∧ ∃ (llen_res : Z),
+ ∧ ∃ llen_res,
    llen_rel v llen_res
-   ∧ ∃ (llen_res_2 : Z),
+   ∧ ∃ llen_res_2,
      llen_rel ⌊ xs ⌋ llen_res_2
-     ∧ ∃ (llen_res_3 : Z),
+     ∧ ∃ llen_res_3,
        llen_rel ⌊ ys ⌋ llen_res_3
-       ∧ ∃ (addZ_res : Z),
+       ∧ ∃ addZ_res,
          addZ_rel llen_res_2 llen_res_3 addZ_res ∧ llen_res == addZ_res) x_62265989 v_x_62265989)).
 Proof.
   buildPackG append append_rel append__append_rel append_rel_funct.
@@ -390,8 +389,7 @@ Defined.
 
 Definition get_spec
   (xs : IList)
-  (i : {i: Z | lebZ_rel 0 i true
-               ∧ ∃ (llen_res : Z), llen_rel ⌊ xs ⌋ llen_res ∧ ltbZ_rel i llen_res true}):
+  (i : {i: Z | lebZ_rel 0 i true ∧ ∃ llen_res, llen_rel ⌊ xs ⌋ llen_res ∧ ltbZ_rel i llen_res true}):
   Type :=
   {v: Z | ltbZ_rel 5 v true}.
 
@@ -399,25 +397,25 @@ Definition get_spec
 
 Definition get
   (xs : IList)
-  (i : {i: Z | lebZ_rel 0 i true
-               ∧ ∃ (llen_res : Z), llen_rel ⌊ xs ⌋ llen_res ∧ ltbZ_rel i llen_res true}):
+  (i : {i: Z | lebZ_rel 0 i true ∧ ∃ llen_res, llen_rel ⌊ xs ⌋ llen_res ∧ ltbZ_rel i llen_res true}):
   get_spec xs i.
 Proof.
   destruct xs as [xs xs_p].
   destruct i as [i i_p].
   try revert i_p; generalize dependent i; induction xs as [x xs' IH_xs'|]; intros.
   - let E := fresh "E" in destruct (i ==? 0) as [|] eqn:E;
-    [refine (IH_xs' ltac:(try clear IH_xs'; solver) (i - 1) ltac:(try clear IH_xs'; solver)) |
-     refine (exist (λ (n : Z), ltbZ_rel 5 n true) x ltac:(solver))].
+    [refine (exist (λ (n : Z), ltbZ_rel 5 n true) x ltac:(solver))|
+     refine (IH_xs' ltac:(try clear IH_xs'; solver) (i - 1) ltac:(try clear IH_xs'; solver))
+     ].
   - intros; exfalso; solver.
 Defined.
 
 Inductive get_rel: IList_u → Z → Z → Prop :=
   | get_Cons_x_False: ∀ x xs' i,
                       (i ==? 0) == false
-                      → ∀ (subZ_res : Z),
+                      → ∀ subZ_res,
                         subZ_rel i 1 subZ_res
-                        → ∀ (get_res : Z), get_rel xs' subZ_res get_res → get_rel (Cons_u x xs') i get_res
+                        → ∀ get_res, get_rel xs' subZ_res get_res → get_rel (Cons_u x xs') i get_res
   | get_Cons_x_True: ∀ x xs' i, (i ==? 0) == true → get_rel (Cons_u x xs') i x.
 
 #[global] Hint Constructors get_rel: core_hint_db.
@@ -439,10 +437,9 @@ Qed.
 Theorem get_Cons_x_lem i x xs' get_Cons_x_lem_res:
   get_rel (Cons_u x xs') i get_Cons_x_lem_res
   ↔ ((i ==? 0) == false
-     → ∃ (subZ_res : Z),
-       subZ_rel i 1 subZ_res
-       ∧ ∃ (get_res : Z), get_rel xs' subZ_res get_res ∧ get_Cons_x_lem_res == get_res)
-    ∨ ((i ==? 0) == true → get_Cons_x_lem_res == x).
+     ∧ ∃ subZ_res,
+       subZ_rel i 1 subZ_res ∧ ∃ get_res, get_rel xs' subZ_res get_res ∧ get_Cons_x_lem_res == get_res)
+    ∨ ((i ==? 0) == true ∧ get_Cons_x_lem_res == x).
 Proof.
   rel_back' ((i ==? 0) _::_ _nil).
 Qed.
@@ -453,20 +450,21 @@ Theorem get_rel_ex
   (xs : IList_u)
   (xs_p : IList_wf xs ∧ True)
   (i : Z)
-  (i_p : lebZ_rel 0 i true ∧ ∃ (llen_res : Z), llen_rel xs llen_res ∧ ltbZ_rel i llen_res true):
+  (i_p : lebZ_rel 0 i true ∧ ∃ llen_res, llen_rel xs llen_res ∧ ltbZ_rel i llen_res true):
   get_rel xs i ⌊ get (exist _ xs xs_p) (exist _ i i_p) -⌋.
 Proof.
   Opaque get.
   existence_lemma_pre get;
   try revert i_p; generalize dependent i; induction xs as [x xs' IH_xs'|]; intros;
   [let E := fresh "E" in destruct (i ==? 0) as [|] eqn:E;
-   [fix_notations;
+   [fix_notations |
+    fix_notations;
     pose proof (IH_xs'
                 ltac:(try clear IH_xs'; solver)
                 (i - 1)
                 ltac:(try clear IH_xs'; solver)) as IH_79916954;
-    try clear IH_xs' |
-    fix_notations] |];
+    try clear IH_xs'
+    ] |];
   simpl in *.
   Transparent get.
   all: (existence_lemma_quicksolve get; f__f_rel_ex_body; f_rel_finish).
@@ -480,7 +478,7 @@ Theorem get__get_rel_rw
   (xs : IList_u)
   (xs_p : IList_wf xs ∧ True)
   (i : Z)
-  (i_p : lebZ_rel 0 i true ∧ ∃ (llen_res : Z), llen_rel xs llen_res ∧ ltbZ_rel i llen_res true)
+  (i_p : lebZ_rel 0 i true ∧ ∃ llen_res, llen_rel xs llen_res ∧ ltbZ_rel i llen_res true)
   (v : Z):
   ⌊ get (exist _ xs xs_p) (exist _ i i_p) -⌋ = v ↔ get_rel xs i v.
 Proof.
@@ -495,8 +493,7 @@ Qed.
 
 Theorem get__get_rel
   (xs : IList)
-  (i : {i: Z | lebZ_rel 0 i true
-               ∧ ∃ (llen_res : Z), llen_rel ⌊ xs ⌋ llen_res ∧ ltbZ_rel i llen_res true})
+  (i : {i: Z | lebZ_rel 0 i true ∧ ∃ llen_res, llen_rel ⌊ xs ⌋ llen_res ∧ ltbZ_rel i llen_res true})
   (v : Z):
   ⌊ get xs i -⌋ = v ↔ get_rel ⌊ xs ⌋ ⌊ i ⌋ v.
 Proof.
@@ -509,8 +506,7 @@ Theorem get__get_rel'
   (xs_u : IList_u)
   (i_u : Z)
   (xs : IList)
-  (i : {i: Z | lebZ_rel 0 i true
-               ∧ ∃ (llen_res : Z), llen_rel ⌊ xs ⌋ llen_res ∧ ltbZ_rel i llen_res true})
+  (i : {i: Z | lebZ_rel 0 i true ∧ ∃ llen_res, llen_rel ⌊ xs ⌋ llen_res ∧ ltbZ_rel i llen_res true})
   (v : Z):
   xs_u = ⌊ xs ⌋ → (i_u = ⌊ i ⌋ → ⌊ get xs i -⌋ = v ↔ get_rel xs_u i_u v).
 Proof.
@@ -523,7 +519,7 @@ Theorem get_rel_mk
   (xs : IList_u)
   (xs_p : IList_wf xs ∧ True)
   (i : Z)
-  (i_p : lebZ_rel 0 i true ∧ ∃ (llen_res : Z), llen_rel xs llen_res ∧ ltbZ_rel i llen_res true):
+  (i_p : lebZ_rel 0 i true ∧ ∃ llen_res, llen_rel xs llen_res ∧ ltbZ_rel i llen_res true):
   {v: _ | get_rel xs i v}.
 Proof.
   intros;
@@ -538,36 +534,34 @@ Qed.
   @Pack
   (IList
    ::RT λ (xs : IList),
-        {i: Z | lebZ_rel 0 i true ∧ ∃ (llen_res : Z), llen_rel ⌊ xs ⌋ llen_res ∧ ltbZ_rel i llen_res true}
+        {i: Z | lebZ_rel 0 i true ∧ ∃ llen_res, llen_rel ⌊ xs ⌋ llen_res ∧ ltbZ_rel i llen_res true}
         ::RT λ (i : {i: Z | lebZ_rel 0 i true
-                            ∧ ∃ (llen_res : Z), llen_rel ⌊ xs ⌋ llen_res ∧ ltbZ_rel i llen_res true}),
+                            ∧ ∃ llen_res, llen_rel ⌊ xs ⌋ llen_res ∧ ltbZ_rel i llen_res true}),
              nilRT)
   (IList_u ::UT (Z ::UT nilUT))
   ltac:(mkProjectsArgListTG ((IList
   ::RT λ (xs : IList),
        {i: Z | lebZ_rel 0 i true
-               ∧ ∃ (llen_res : Z),
-                 llen_rel ⌊ xs ⌋ llen_res ∧ ltbZ_rel i llen_res true}
+               ∧ ∃ llen_res, llen_rel ⌊ xs ⌋ llen_res ∧ ltbZ_rel i llen_res true}
        ::RT λ (i : {i: Z | lebZ_rel 0 i true
-                           ∧ ∃ (llen_res : Z),
+                           ∧ ∃ llen_res,
                              llen_rel ⌊ xs ⌋ llen_res ∧ ltbZ_rel i llen_res true}),
             nilRT)) ((IList_u ::UT (Z ::UT nilUT))))
   Z
-  (λ (x_12457766 : ArgList (IList
+  (λ (x_20044467 : ArgList (IList
                             ::RT λ (xs : IList),
                                  {i: Z | lebZ_rel 0 i true
-                                         ∧ ∃ (llen_res : Z), llen_rel ⌊ xs ⌋ llen_res ∧ ltbZ_rel i llen_res true}
+                                         ∧ ∃ llen_res, llen_rel ⌊ xs ⌋ llen_res ∧ ltbZ_rel i llen_res true}
                                  ::RT λ (i : {i: Z | lebZ_rel 0 i true
-                                                     ∧ ∃ (llen_res : Z),
+                                                     ∧ ∃ llen_res,
                                                        llen_rel ⌊ xs ⌋ llen_res ∧ ltbZ_rel i llen_res true}),
                                       nilRT))
-     (v_x_12457766 : Z),
+     (v_x_20044467 : Z),
    ltac:(flattenP (λ (xs : IList)
    (i : {i: Z | lebZ_rel 0 i true
-                ∧ ∃ (llen_res : Z),
-                  llen_rel ⌊ xs ⌋ llen_res ∧ ltbZ_rel i llen_res true})
+                ∧ ∃ llen_res, llen_rel ⌊ xs ⌋ llen_res ∧ ltbZ_rel i llen_res true})
    (v : Z),
- ltbZ_rel 5 v true) x_12457766 v_x_12457766)).
+ ltbZ_rel 5 v true) x_20044467 v_x_20044467)).
 Proof.
   buildPackG get get_rel get__get_rel get_rel_funct.
 Defined.
@@ -585,10 +579,9 @@ Definition applyToFirst_spec
        Z
        (λ (x_46517173 : ArgList ({VV: Z | True} ::RT λ (f : {VV: Z | True}), nilRT)) (v_x_46517173 : Z),
         ltac:(flattenP (λ (f : {VV: Z | True}) (y : Z), ltbZ_rel 5 y true) x_46517173 v_x_46517173)))
-  (xs : {xs: IList_u | IList_wf xs ∧ ∃ (llen_res : Z), llen_rel xs llen_res ∧ llen_res ≠ 0}):
+  (xs : {xs: IList_u | IList_wf xs ∧ ∃ llen_res, llen_rel xs llen_res ∧ llen_res ≠ 0}):
   Type :=
-  {v: Z | ∃ (get_res : Z),
-          get_rel ⌊ xs ⌋ 0 get_res ∧ ∃ (f_res : Z), getPackRel f get_res f_res ∧ v == f_res}.
+  {v: Z | ∃ get_res, get_rel ⌊ xs ⌋ 0 get_res ∧ ∃ f_res, getPackRel f get_res f_res ∧ v == f_res}.
 
 #[global] Hint Unfold applyToFirst_spec: lia_unfold.
 
@@ -600,27 +593,26 @@ Definition applyToFirst
        Z
        (λ (x_46517173 : ArgList ({VV: Z | True} ::RT λ (f : {VV: Z | True}), nilRT)) (v_x_46517173 : Z),
         ltac:(flattenP (λ (f : {VV: Z | True}) (y : Z), ltbZ_rel 5 y true) x_46517173 v_x_46517173)))
-  (xs : {xs: IList_u | IList_wf xs ∧ ∃ (llen_res : Z), llen_rel xs llen_res ∧ llen_res ≠ 0}):
+  (xs : {xs: IList_u | IList_wf xs ∧ ∃ llen_res, llen_rel xs llen_res ∧ llen_res ≠ 0}):
   applyToFirst_spec f xs.
 Proof.
   destruct xs as [xs xs_p].
   destruct xs as [x l'|].
   - refine (subsumptionCast
             Z
-            (λ (v : Z),
-             ∃ (get_res : Z), get_rel xs 0 get_res ∧ ∃ (f_res : Z), getPackRel f get_res f_res ∧ v == f_res)
+            (λ (v : Z), ∃ get_res, get_rel (Cons_u x l') 0 get_res ∧ ∃ (f_res : Z), getPackRel f get_res f_res ∧ v == f_res)
             (getPackF f
              (subsumptionCast
               Z
               (λ (VV : Z), True)
               (exist (λ (n : Z), ltbZ_rel 5 n true) x ltac:(solver))
               ltac:(solver)))
-            ltac:(solver)).
+            ltac:(time solver)).
   - intros; exfalso; solver.
 Defined.
 
 Inductive applyToFirst_rel: @uPack (Z ::UT nilUT) Z → IList_u → Z → Prop :=
-  | applyToFirst_x_Cons: ∀ (f : @uPack (Z ::UT nilUT) Z) l' x (f_res : Z),
+  | applyToFirst_x_Cons: ∀ (f : @uPack (Z ::UT nilUT) Z) l' x f_res,
                          getUPackRel f x f_res → applyToFirst_rel f (Cons_u x l') f_res.
 
 #[global] Hint Constructors applyToFirst_rel: core_hint_db.
@@ -640,7 +632,7 @@ Qed.
 
 Theorem applyToFirst_x_Cons_lem f l' x applyToFirst_x_Cons_lem_res:
   applyToFirst_rel f (Cons_u x l') applyToFirst_x_Cons_lem_res
-  ↔ ∃ (f_res : Z), getUPackRel f x f_res ∧ applyToFirst_x_Cons_lem_res == f_res.
+  ↔ ∃ f_res, getUPackRel f x f_res ∧ applyToFirst_x_Cons_lem_res == f_res.
 Proof.
   rel_back' _nil.
 Qed.
@@ -656,7 +648,7 @@ Theorem applyToFirst_rel_ex
        (λ (x_30423934 : ArgList ({f: Z | True} ::RT λ (f : {f: Z | True}), nilRT)) (v_x_30423934 : Z),
         ltac:(flattenP (λ (f : {f: Z | True}) (y : Z), ltbZ_rel 5 y true) x_30423934 v_x_30423934)))
   (xs : IList_u)
-  (xs_p : IList_wf xs ∧ ∃ (llen_res : Z), llen_rel xs llen_res ∧ llen_res ≠ 0):
+  (xs_p : IList_wf xs ∧ ∃ llen_res, llen_rel xs llen_res ∧ llen_res ≠ 0):
   applyToFirst_rel ⌊ f ⌋ xs ⌊ applyToFirst f (exist _ xs xs_p) -⌋.
 Proof.
   Opaque applyToFirst.
@@ -681,7 +673,7 @@ Theorem applyToFirst__applyToFirst_rel_rw
        (λ (x_30423934 : ArgList ({f: Z | True} ::RT λ (f : {f: Z | True}), nilRT)) (v_x_30423934 : Z),
         ltac:(flattenP (λ (f : {f: Z | True}) (y : Z), ltbZ_rel 5 y true) x_30423934 v_x_30423934)))
   (xs : IList_u)
-  (xs_p : IList_wf xs ∧ ∃ (llen_res : Z), llen_rel xs llen_res ∧ llen_res ≠ 0)
+  (xs_p : IList_wf xs ∧ ∃ llen_res, llen_rel xs llen_res ∧ llen_res ≠ 0)
   (v : Z):
   ⌊ applyToFirst f (exist _ xs xs_p) -⌋ = v ↔ applyToFirst_rel ⌊ f ⌋ xs v.
 Proof.
@@ -703,7 +695,7 @@ Theorem applyToFirst__applyToFirst_rel
        Z
        (λ (x_46517173 : ArgList ({VV: Z | True} ::RT λ (f : {VV: Z | True}), nilRT)) (v_x_46517173 : Z),
         ltac:(flattenP (λ (f : {VV: Z | True}) (y : Z), ltbZ_rel 5 y true) x_46517173 v_x_46517173)))
-  (xs : {xs: IList_u | IList_wf xs ∧ ∃ (llen_res : Z), llen_rel xs llen_res ∧ llen_res ≠ 0})
+  (xs : {xs: IList_u | IList_wf xs ∧ ∃ llen_res, llen_rel xs llen_res ∧ llen_res ≠ 0})
   (v : Z):
   ⌊ applyToFirst f xs -⌋ = v ↔ applyToFirst_rel ⌊ f ⌋ ⌊ xs ⌋ v.
 Proof.
@@ -722,7 +714,7 @@ Theorem applyToFirst__applyToFirst_rel'
        Z
        (λ (x_46517173 : ArgList ({VV: Z | True} ::RT λ (f : {VV: Z | True}), nilRT)) (v_x_46517173 : Z),
         ltac:(flattenP (λ (f : {VV: Z | True}) (y : Z), ltbZ_rel 5 y true) x_46517173 v_x_46517173)))
-  (xs : {xs: IList_u | IList_wf xs ∧ ∃ (llen_res : Z), llen_rel xs llen_res ∧ llen_res ≠ 0})
+  (xs : {xs: IList_u | IList_wf xs ∧ ∃ llen_res, llen_rel xs llen_res ∧ llen_res ≠ 0})
   (v : Z):
   f_u = ⌊ f ⌋ → (xs_u = ⌊ xs ⌋ → ⌊ applyToFirst f xs -⌋ = v ↔ applyToFirst_rel f_u xs_u v).
 Proof.
@@ -740,7 +732,7 @@ Theorem applyToFirst_rel_mk
        (λ (x_30423934 : ArgList ({f: Z | True} ::RT λ (f : {f: Z | True}), nilRT)) (v_x_30423934 : Z),
         ltac:(flattenP (λ (f : {f: Z | True}) (y : Z), ltbZ_rel 5 y true) x_30423934 v_x_30423934)))
   (xs : IList_u)
-  (xs_p : IList_wf xs ∧ ∃ (llen_res : Z), llen_rel xs llen_res ∧ llen_res ≠ 0):
+  (xs_p : IList_wf xs ∧ ∃ llen_res, llen_rel xs llen_res ∧ llen_res ≠ 0):
   {v: _ | applyToFirst_rel (packProj f) xs v}.
 Proof.
   intros;
@@ -758,22 +750,20 @@ Qed.
 Definition thm1_spec
   (xs : IList)
   (x : {x: Z | ltbZ_rel 5 x true})
-  (i : {i: Z | lebZ_rel 0 i true
-               ∧ ∃ (llen_res : Z), llen_rel ⌊ xs ⌋ llen_res ∧ ltbZ_rel i llen_res true}):
+  (i : {i: Z | lebZ_rel 0 i true ∧ ∃ llen_res, llen_rel ⌊ xs ⌋ llen_res ∧ ltbZ_rel i llen_res true}):
   Type :=
-  {{∃ (get_res : Z),
+  {{∃ get_res,
     get_rel ⌊ xs ⌋ ⌊ i ⌋ get_res
-    ∧ ∃ (addZ_res : Z),
+    ∧ ∃ addZ_res,
       addZ_rel ⌊ i ⌋ 1 addZ_res
-      ∧ ∃ (get_res_2 : Z), get_rel (Cons_u ⌊ x ⌋ ⌊ xs ⌋) addZ_res get_res_2 ∧ get_res == get_res_2}}.
+      ∧ ∃ get_res_2, get_rel (Cons_u ⌊ x ⌋ ⌊ xs ⌋) addZ_res get_res_2 ∧ get_res == get_res_2}}.
 
 #[global] Hint Unfold thm1_spec: lia_unfold.
 
 Theorem thm1
   (xs : IList)
   (x : {x: Z | ltbZ_rel 5 x true})
-  (i : {i: Z | lebZ_rel 0 i true
-               ∧ ∃ (llen_res : Z), llen_rel ⌊ xs ⌋ llen_res ∧ ltbZ_rel i llen_res true}):
+  (i : {i: Z | lebZ_rel 0 i true ∧ ∃ llen_res, llen_rel ⌊ xs ⌋ llen_res ∧ ltbZ_rel i llen_res true}):
   thm1_spec xs x i.
 Proof.
   destruct xs as [xs xs_p].
@@ -782,36 +772,34 @@ Proof.
   refine (subsumptionCast
           Unit
           (λ (VV : Unit),
-           ∃ (get_res : Z),
+           ∃ get_res,
            get_rel xs i get_res
-           ∧ ∃ (addZ_res : Z),
+           ∧ ∃ addZ_res,
              addZ_rel i 1 addZ_res
-             ∧ ∃ (get_res_2 : Z), get_rel (Cons_u x xs) addZ_res get_res_2 ∧ get_res == get_res_2)
+             ∧ ∃ get_res_2, get_rel (Cons_u x xs) addZ_res get_res_2 ∧ get_res == get_res_2)
           (# unit)
           ltac:(solver)).
 Qed.
 
 Definition thm2_spec
   (xs ys : IList)
-  (i : {i: Z | lebZ_rel 0 i true
-               ∧ ∃ (llen_res : Z), llen_rel ⌊ xs ⌋ llen_res ∧ ltbZ_rel i llen_res true}):
+  (i : {i: Z | lebZ_rel 0 i true ∧ ∃ llen_res, llen_rel ⌊ xs ⌋ llen_res ∧ ltbZ_rel i llen_res true}):
   Type :=
-  {{∃ (get_res : Z),
+  {{∃ get_res,
     get_rel ⌊ xs ⌋ ⌊ i ⌋ get_res
-    ∧ ∃ (llen_res : Z),
+    ∧ ∃ llen_res,
       llen_rel ⌊ ys ⌋ llen_res
-      ∧ ∃ (addZ_res : Z),
+      ∧ ∃ addZ_res,
         addZ_rel ⌊ i ⌋ llen_res addZ_res
-        ∧ ∃ (append_res : IList_u),
+        ∧ ∃ append_res,
           append_rel ⌊ ys ⌋ ⌊ xs ⌋ append_res
-          ∧ ∃ (get_res_2 : Z), get_rel append_res addZ_res get_res_2 ∧ get_res == get_res_2}}.
+          ∧ ∃ get_res_2, get_rel append_res addZ_res get_res_2 ∧ get_res == get_res_2}}.
 
 #[global] Hint Unfold thm2_spec: lia_unfold.
 
 Theorem thm2
   (xs ys : IList)
-  (i : {i: Z | lebZ_rel 0 i true
-               ∧ ∃ (llen_res : Z), llen_rel ⌊ xs ⌋ llen_res ∧ ltbZ_rel i llen_res true}):
+  (i : {i: Z | lebZ_rel 0 i true ∧ ∃ llen_res, llen_rel ⌊ xs ⌋ llen_res ∧ ltbZ_rel i llen_res true}):
   thm2_spec xs ys i.
 Proof.
   destruct xs as [xs xs_p].
@@ -823,25 +811,25 @@ Proof.
   - refine (subsumptionCast
             Unit
             (λ (VV : Unit),
-             ∃ (get_res : Z),
+             ∃ get_res,
              get_rel xs i get_res
-             ∧ ∃ (llen_res : Z),
+             ∧ ∃ llen_res,
                llen_rel ys llen_res
-               ∧ ∃ (addZ_res : Z),
+               ∧ ∃ addZ_res,
                  addZ_rel i llen_res addZ_res
-                 ∧ ∃ (append_res : IList_u),
+                 ∧ ∃ append_res,
                    append_rel ys xs append_res
-                   ∧ ∃ (get_res_2 : Z), get_rel append_res addZ_res get_res_2 ∧ get_res == get_res_2)
-            (let _: ∃ (get_res : Z),
+                   ∧ ∃ get_res_2, get_rel append_res addZ_res get_res_2 ∧ get_res == get_res_2)
+            (let _: ∃ get_res,
                     get_rel
                     ⌊ append
                       (exist (λ (l : IList_u), IList_wf l ∧ True) ys ltac:(solver))
                       (exist (λ (xs : IList_u), IList_wf xs ∧ True) xs ltac:(solver)) ⌋
                     (i + ⌊ llen (exist (λ (l : IList_u), IList_wf l ∧ True) ys ltac:(solver)) ⌋)
                     get_res
-                    ∧ ∃ (addZ_res : Z),
+                    ∧ ∃ addZ_res,
                       addZ_rel (i + ⌊ llen (exist (λ (l : IList_u), IList_wf l ∧ True) ys ltac:(solver)) ⌋) 1 addZ_res
-                      ∧ ∃ (get_res_2 : Z),
+                      ∧ ∃ get_res_2,
                         get_rel
                         (Cons_u y
                          ⌊ append
@@ -863,7 +851,7 @@ Proof.
                 Z
                 (λ (i : Z),
                  lebZ_rel 0 i true
-                 ∧ ∃ (llen_res : Z),
+                 ∧ ∃ llen_res,
                    llen_rel
                    ⌊ append
                      (exist (λ (l : IList_u), IList_wf l ∧ True) ys ltac:(solver))
@@ -875,7 +863,7 @@ Proof.
                  (λ (x_1 : Z), True)
                  (exist (λ (i : Z),
                          lebZ_rel 0 i true
-                         ∧ ∃ (llen_res : Z), llen_rel xs llen_res ∧ ltbZ_rel i llen_res true) i ltac:(solver))
+                         ∧ ∃ llen_res, llen_rel xs llen_res ∧ ltbZ_rel i llen_res true) i ltac:(solver))
                  ltac:(solver)
                  +Z subsumptionCast
                     Z
@@ -893,15 +881,15 @@ Proof.
   - refine (subsumptionCast
             Unit
             (λ (VV : Unit),
-             ∃ (get_res : Z),
+             ∃ get_res,
              get_rel xs i get_res
-             ∧ ∃ (llen_res : Z),
+             ∧ ∃ llen_res,
                llen_rel ys llen_res
-               ∧ ∃ (addZ_res : Z),
+               ∧ ∃ addZ_res,
                  addZ_rel i llen_res addZ_res
-                 ∧ ∃ (append_res : IList_u),
+                 ∧ ∃ append_res,
                    append_rel ys xs append_res
-                   ∧ ∃ (get_res_2 : Z), get_rel append_res addZ_res get_res_2 ∧ get_res == get_res_2)
+                   ∧ ∃ get_res_2, get_rel append_res addZ_res get_res_2 ∧ get_res == get_res_2)
             (# unit)
             ltac:(solver)).
 Qed.
